thys/examples/code/exp.h
@@ -5,6 +5,8 @@
 
 
 
+
+
 uint64_t exp64(uint64_t);
 uint32_t exp32(uint32_t);
 
