thys/ds/LLVM_DS_All.thy
@@ -1,0 +1,18 @@
+theory LLVM_DS_All
+imports
+  Array_of_Array_List
+  LLVM_DS_Arith
+  LLVM_DS_Array_List_Pure
+  LLVM_DS_Array_List
+  LLVM_DS_Array
+  LLVM_DS_Block_Alloc
+  LLVM_DS_Circ_List
+  LLVM_DS_Dflt
+  LLVM_DS_List_Assn
+  LLVM_DS_List_Seg
+  LLVM_DS_NArray
+  LLVM_DS_Open_List
+  Proto_EOArray
+begin
+
+end
